core/minted.v
@@ -1,0 +1,123 @@
+From mathcomp Require Import ssreflect.
+From stdpp Require Import gmap.
+From iris.algebra Require Import agree auth gset gmap list reservation_map excl.
+From iris.algebra Require Import functions.
+From iris.base_logic.lib Require Import saved_prop invariants.
+From iris.heap_lang Require Import notation proofmode.
+From cryptis Require Import lib gmeta nown.
+From cryptis.core Require Import term.
+
+Set Implicit Arguments.
+Unset Strict Implicit.
+Unset Printing Implicit Defensive.
+
+Section Minted.
+
+Context `{heapGS Σ}.
+
+Notation iProp := (iProp Σ).
+
+Fact minted_key : unit. Proof. exact: tt. Qed.
+
+Definition minted : term → iProp :=
+  locked_with minted_key (
+    λ t, [∗ set] a ∈ nonces_of_term t,
+      meta a (nroot.@"minted") ()
+  )%I.
+
+Canonical minted_unlock := [unlockable of minted].
+
+Global Instance Persistent_minted t : Persistent (minted t).
+Proof. rewrite unlock; apply _. Qed.
+
+Global Instance Timeless_minted t : Timeless (minted t).
+Proof. rewrite unlock; apply _. Qed.
+
+Lemma subterm_minted t1 t2 :
+  subterm t1 t2 → minted t2 -∗ minted t1.
+Proof.
+rewrite unlock !big_sepS_forall; iIntros "%sub m_t2 %t %t_t1".
+move/subterm_nonces_of_term in sub.
+iApply "m_t2". iPureIntro. set_solver.
+Qed.
+
+Lemma minted_TInt n : minted (TInt n) ⊣⊢ True.
+Proof. by rewrite unlock nonces_of_term_unseal /= big_sepS_empty. Qed.
+
+Lemma minted_TPair t1 t2 : minted (TPair t1 t2) ⊣⊢ minted t1 ∧ minted t2.
+Proof.
+by rewrite unlock nonces_of_term_unseal /= !big_sepS_union_pers.
+Qed.
+
+Lemma minted_TNonce a : minted (TNonce a) ⊣⊢ meta a (nroot.@"minted") ().
+Proof.
+by rewrite unlock nonces_of_term_unseal /= big_sepS_singleton.
+Qed.
+
+Lemma minted_TKey kt t : minted (TKey kt t) ⊣⊢ minted t.
+Proof. by rewrite unlock nonces_of_term_unseal /=. Qed.
+
+Lemma minted_TEnc k t : minted (TEnc k t) ⊣⊢ minted k ∧ minted t.
+Proof.
+by rewrite unlock nonces_of_term_unseal /= !big_sepS_union_pers.
+Qed.
+
+Lemma minted_THash t : minted (THash t) ⊣⊢ minted t.
+Proof. by rewrite unlock nonces_of_term_unseal /=. Qed.
+
+Lemma minted_TExpN t ts :
+  minted (TExpN t ts) ⊣⊢ minted t ∧ [∗ list] t' ∈ ts, minted t'.
+Proof.
+rewrite unlock nonces_of_term_TExpN big_sepS_union_pers.
+by rewrite big_sepS_union_list_pers big_sepL_fmap.
+Qed.
+
+Lemma minted_TExp t1 t2 :
+  minted (TExp t1 t2) ⊣⊢ minted t1 ∧ minted t2.
+Proof.
+rewrite unlock nonces_of_term_TExpN big_sepS_union_pers.
+by rewrite /= union_empty_r_L.
+Qed.
+
+Lemma minted_nonces_of_term t :
+  minted t ⊣⊢ [∗ set] a ∈ nonces_of_term t, minted (TNonce a).
+Proof.
+rewrite {1}unlock !big_sepS_forall; iSplit; iIntros "#H %a %a_t".
+- by rewrite minted_TNonce; iApply "H".
+- by rewrite -minted_TNonce; iApply "H".
+Qed.
+
+Lemma minted_to_list t ts :
+  Spec.to_list t = Some ts →
+  minted t -∗ [∗ list] t' ∈ ts, minted t'.
+Proof.
+elim/term_ind': t ts => //=.
+  by case=> // ts [<-] /=; iIntros "?".
+move=> t _ tl IH ts.
+case e: (Spec.to_list tl) => [ts'|] // [<-] /=.
+rewrite minted_TPair /=; iIntros "[??]"; iFrame.
+by iApply IH.
+Qed.
+
+Lemma minted_of_list ts :
+  minted (Spec.of_list ts) ⊣⊢
+  [∗ list] t ∈ ts, minted t.
+Proof.
+rewrite Spec.of_list_unseal.
+elim: ts => [|t ts IH]; first by rewrite minted_TInt.
+by rewrite minted_TPair /= IH bi.persistent_and_sep.
+Qed.
+
+Lemma minted_tag N t : minted (Spec.tag N t) ⊣⊢ minted t.
+Proof.
+by rewrite Spec.tag_unseal minted_TPair minted_TInt bi.emp_and.
+Qed.
+
+Lemma minted_mkskey k : minted (Spec.mkskey k) ⊣⊢ minted k.
+Proof.
+rewrite minted_TPair !minted_TKey !minted_tag.
+iSplit; [iIntros "[_ ?]"|]; eauto.
+Qed.
+
+End Minted.
+
