core/public.v
@@ -1,0 +1,980 @@
+From mathcomp Require Import ssreflect.
+From stdpp Require Import gmap.
+From iris.algebra Require Import agree auth gset gmap list reservation_map excl.
+From iris.algebra Require Import functions.
+From iris.base_logic.lib Require Import saved_prop invariants.
+From iris.heap_lang Require Import notation proofmode.
+From cryptis Require Import lib.
+From cryptis.core Require Import term minted.
+
+Set Implicit Arguments.
+Unset Strict Implicit.
+Unset Printing Implicit Defensive.
+
+Class publicGpreS Σ := PublicGPreS {
+  publicGpreS_nonce : savedPredG Σ term;
+  publicGpreS_key   : savedPredG Σ (key_type * term);
+  publicGpreS_enc   : savedPredG Σ (term * term);
+  (* TODO: Replace this with metaGS *)
+  publicGpreS_maps  : inG Σ (reservation_mapR (agreeR positiveO));
+}.
+
+Local Existing Instance publicGpreS_nonce.
+Local Existing Instance publicGpreS_key.
+Local Existing Instance publicGpreS_enc.
+Local Existing Instance publicGpreS_maps.
+
+Class publicGS Σ := PublicGS {
+  public_inG : publicGpreS Σ;
+  public_key_name   : gname;
+  public_hash_name  : gname;
+  public_enc_name   : gname;
+}.
+
+Global Existing Instance public_inG.
+
+Definition publicΣ : gFunctors :=
+  #[savedPredΣ term;
+    savedPredΣ (key_type * term);
+    savedPredΣ (term * term);
+    GFunctor (reservation_mapR (agreeR positiveO))].
+
+Global Instance subG_publicGpreS Σ : subG publicΣ Σ → publicGpreS Σ.
+Proof. solve_inG. Qed.
+
+Section Public.
+
+Context `{!heapGS Σ, !publicGS Σ}.
+Notation iProp := (iProp Σ).
+Notation iPropO := (iPropO Σ).
+Notation iPropI := (iPropI Σ).
+
+Definition pnonce a : iProp :=
+  ∃ γ P, meta a (nroot.@"nonce") γ ∧
+         saved_pred_own γ DfracDiscarded P ∧
+         ▷ □ P (TNonce a).
+
+Global Instance Persistent_pnonce a : Persistent (pnonce a).
+Proof. apply _. Qed.
+
+Definition dh_pred (t t' : term) : iProp :=
+  match t with
+  | TNonce a =>
+    ∃ γ φ, meta a (nroot.@"dh") γ ∧
+           saved_pred_own γ DfracDiscarded φ ∧
+           ▷ □ φ t'
+  | _ => False
+  end.
+
+Global Instance Persistent_dh_pred t t' : Persistent (dh_pred t t').
+Proof. case: t => *; apply _. Qed.
+
+Definition enc_pred N Φ : iProp :=
+  ∃ γ, own public_enc_name (namespace_map_data N (to_agree γ)) ∧
+       saved_pred_own γ DfracDiscarded (fun '(k, t) => Φ k t).
+
+Definition enc_pred_token E :=
+  own public_enc_name (reservation_map_token E).
+
+Lemma enc_pred_token_difference E1 E2 :
+  E1 ⊆ E2 →
+  enc_pred_token E2 ⊣⊢ enc_pred_token E1 ∗ enc_pred_token (E2 ∖ E1).
+Proof.
+move=> sub; rewrite /enc_pred_token.
+by rewrite (reservation_map_token_difference E1 E2) // own_op.
+Qed.
+
+Lemma enc_pred_token_drop E1 E2 :
+  E1 ⊆ E2 →
+  enc_pred_token E2 -∗
+  enc_pred_token E1.
+Proof.
+iIntros (sub) "t".
+rewrite enc_pred_token_difference //.
+by iDestruct "t" as "[t _]".
+Qed.
+
+Global Instance enc_pred_persistent N Φ : Persistent (enc_pred N Φ).
+Proof. apply _. Qed.
+
+Lemma enc_pred_agree k t N Φ1 Φ2 :
+  enc_pred N Φ1 -∗
+  enc_pred N Φ2 -∗
+  ▷ (Φ1 k t ≡ Φ2 k t).
+Proof.
+iDestruct 1 as (γm1) "[#meta1 #own1]".
+iDestruct 1 as (γm2) "[#meta2 #own2]".
+iPoseProof (own_valid_2 with "meta1 meta2") as "%valid".
+move: valid; rewrite -reservation_map_data_op reservation_map_data_valid.
+move=> /to_agree_op_inv_L ->.
+by iApply (saved_pred_agree _ _ _ _ _ (k, t) with "own1 own2").
+Qed.
+
+Lemma enc_pred_set E (N : namespace) Φ :
+  ↑N ⊆ E →
+  enc_pred_token E ==∗
+  enc_pred N Φ ∗
+  enc_pred_token (E ∖ ↑N).
+Proof.
+iIntros (?) "token".
+iMod (saved_pred_alloc (λ '(k, t), Φ k t) DfracDiscarded) as (γ) "own" => //.
+rewrite (@enc_pred_token_difference (↑N)) //.
+iDestruct "token" as "[token ?]".
+iMod (own_update with "token").
+  eapply (namespace_map_alloc_update _ _ (to_agree γ)) => //.
+by iModIntro; iFrame; iExists γ; iSplit.
+Qed.
+
+Definition wf_enc k t : iProp :=
+  ∃ N t' Φ, ⌜t = Spec.tag N t'⌝ ∧ enc_pred N Φ ∧ □ ▷ Φ k t'.
+
+Global Instance wf_enc_persistent k t : Persistent (wf_enc k t).
+Proof. by apply _. Qed.
+
+Lemma wf_enc_elim k N t Φ :
+  wf_enc k (Spec.tag N t) -∗
+  enc_pred N Φ -∗
+  □ ▷ Φ k t.
+Proof.
+iDestruct 1 as (N' t' Φ') "(%t_t' & #HΦ' & #inv)"; iIntros "#HΦ".
+case/Spec.tag_inj: t_t' => <- <-.
+iPoseProof (enc_pred_agree k t with "HΦ HΦ'") as "e".
+by iIntros "!> !>"; iRewrite "e".
+Qed.
+
+Definition key_pred N (φ : key_type → term → iProp) : iProp :=
+  ∃ γ, own public_key_name (namespace_map_data N (to_agree γ)) ∧
+       saved_pred_own γ DfracDiscarded (λ '(kt, t), φ kt t).
+
+Definition key_pred_token E :=
+  own public_key_name (reservation_map_token E).
+
+Lemma key_pred_token_difference E1 E2 :
+  E1 ⊆ E2 →
+  key_pred_token E2 ⊣⊢ key_pred_token E1 ∗ key_pred_token (E2 ∖ E1).
+Proof.
+move=> sub; rewrite /key_pred_token.
+by rewrite (reservation_map_token_difference E1 E2) // own_op.
+Qed.
+
+Lemma key_pred_token_drop E1 E2 :
+  E1 ⊆ E2 →
+  key_pred_token E2 -∗
+  key_pred_token E1.
+Proof.
+iIntros (sub) "t".
+rewrite key_pred_token_difference //.
+by iDestruct "t" as "[t _]".
+Qed.
+
+Global Instance key_pred_persistent N φ : Persistent (key_pred N φ).
+Proof. apply _. Qed.
+
+Lemma key_pred_agree kt t N P₁ P₂ :
+  key_pred N P₁ -∗
+  key_pred N P₂ -∗
+  ▷ (P₁ kt t ≡ P₂ kt t).
+Proof.
+iDestruct 1 as (γm1) "[#meta1 #own1]".
+iDestruct 1 as (γm2) "[#meta2 #own2]".
+iPoseProof (own_valid_2 with "meta1 meta2") as "%valid".
+move: valid; rewrite -reservation_map_data_op reservation_map_data_valid.
+move=> /to_agree_op_inv_L ->.
+by iApply (saved_pred_agree _ _ _ _ _ (kt, t) with "own1 own2").
+Qed.
+
+Lemma key_pred_set E N P :
+  ↑N ⊆ E →
+  key_pred_token E ==∗
+  key_pred N P ∗
+  key_pred_token (E ∖ ↑N).
+Proof.
+iIntros (?) "token".
+rewrite (@key_pred_token_difference (↑N)) //.
+iDestruct "token" as "[token ?]".
+iMod (saved_pred_alloc (λ '(kt, t), P kt t) DfracDiscarded) as (γ) "own" => //.
+iMod (own_update with "token").
+  by eapply (namespace_map_alloc_update _ _ (to_agree γ)) => //.
+by iModIntro; iFrame; iExists γ; iSplit.
+Qed.
+
+Definition wf_key kt t : iProp :=
+  ∃ N t' P, ⌜t = Spec.tag N t'⌝ ∧ key_pred N P ∧ □ ▷ P kt t'.
+
+Global Instance wf_key_persistent kt t : Persistent (wf_key kt t).
+Proof. by apply _. Qed.
+
+Lemma wf_key_elim N kt t P :
+  wf_key kt (Spec.tag N t) -∗
+  key_pred N P -∗
+  □ ▷ P kt t.
+Proof.
+iDestruct 1 as (N' t' P') "(%t_t' & #HP' & #inv)"; iIntros "#HP".
+case/Spec.tag_inj: t_t' => <- <-.
+iPoseProof (key_pred_agree kt t with "HP HP'") as "e".
+by iIntros "!> !>"; iRewrite "e".
+Qed.
+
+Definition hash_pred N (P : term → iProp) : iProp :=
+  ∃ γ, own public_hash_name (namespace_map_data N (to_agree γ)) ∧
+       saved_pred_own γ DfracDiscarded P.
+
+Definition hash_pred_token E :=
+  own public_hash_name (reservation_map_token E).
+
+Lemma hash_pred_token_difference E1 E2 :
+  E1 ⊆ E2 →
+  hash_pred_token E2 ⊣⊢ hash_pred_token E1 ∗ hash_pred_token (E2 ∖ E1).
+Proof.
+move=> sub; rewrite /hash_pred_token.
+by rewrite (reservation_map_token_difference E1 E2) // own_op.
+Qed.
+
+Lemma hash_pred_token_drop E1 E2 :
+  E1 ⊆ E2 →
+  hash_pred_token E2 -∗
+  hash_pred_token E1.
+Proof.
+iIntros (sub) "t".
+rewrite hash_pred_token_difference //.
+by iDestruct "t" as "[t _]".
+Qed.
+
+Global Instance hash_pred_persistent N P : Persistent (hash_pred N P).
+Proof. apply _. Qed.
+
+Lemma hash_pred_agree t N P₁ P₂ :
+  hash_pred N P₁ -∗
+  hash_pred N P₂ -∗
+  ▷ (P₁ t ≡ P₂ t).
+Proof.
+iDestruct 1 as (γm1) "[#meta1 #own1]".
+iDestruct 1 as (γm2) "[#meta2 #own2]".
+iPoseProof (own_valid_2 with "meta1 meta2") as "%valid".
+move: valid; rewrite -reservation_map_data_op reservation_map_data_valid.
+move=> /to_agree_op_inv_L ->.
+by iApply (saved_pred_agree _ _ _ _ _ t with "own1 own2").
+Qed.
+
+Lemma hash_pred_set E N P :
+  ↑N ⊆ E →
+  hash_pred_token E ==∗
+  hash_pred N P ∗
+  hash_pred_token (E ∖ ↑N).
+Proof.
+iIntros (?) "token".
+rewrite (@hash_pred_token_difference (↑N)) //.
+iDestruct "token" as "[token ?]".
+iMod (saved_pred_alloc P DfracDiscarded) as (γ) "own" => //.
+iMod (own_update with "token").
+  by eapply (namespace_map_alloc_update _ _ (to_agree γ)) => //.
+by iModIntro; iFrame; iExists γ; iSplit.
+Qed.
+
+Definition wf_hash t : iProp :=
+  ∃ N t' P, ⌜t = Spec.tag N t'⌝ ∧ hash_pred N P ∧ □ ▷ P t'.
+
+Global Instance wf_hash_persistent t : Persistent (wf_hash t).
+Proof. by apply _. Qed.
+
+Lemma wf_hash_elim N t P :
+  wf_hash (Spec.tag N t) -∗
+  hash_pred N P -∗
+  □ ▷ P t.
+Proof.
+iDestruct 1 as (N' t' P') "(%t_t' & #HP' & #inv)"; iIntros "#HP".
+case/Spec.tag_inj: t_t' => <- <-.
+iPoseProof (hash_pred_agree t with "HP HP'") as "e".
+by iIntros "!> !>"; iRewrite "e".
+Qed.
+
+Inductive decompose (T : gset term) (t : term) : Prop :=
+| DInt n of T = ∅ & t = TInt n
+
+| DPair t1 t2 of T = {[t1; t2]} & t = TPair t1 t2
+
+| DKey kt t' of T = {[t']} & t = TKey kt t'
+
+| DEnc k t' of T = {[k; t']} & t = TEnc k t'
+
+| DHash t' of T = {[t']} & t = THash t'
+
+| DExp t1 t2 of T = {[t1; t2]} & is_exp t & t = TExp t1 t2.
+
+Lemma decompose_tsize T t t' : decompose T t → t' ∈ T → tsize t' < tsize t.
+Proof.
+case.
+- by move=> n -> -> //.
+- move=> t1 t2 -> ->.
+  case/elem_of_union => /elem_of_singleton ->;
+  rewrite [tsize (TPair _ _)]tsize_eq -ssrnat.plusE; lia.
+- move=> kt ? -> -> /elem_of_singleton ->.
+  rewrite [tsize (TKey _ _)]tsize_eq; lia.
+- move=> ?? -> -> /elem_of_union [] /elem_of_singleton ->;
+  rewrite ?[tsize (TKey _ _)]tsize_eq [tsize (TEnc _ _)]tsize_eq -ssrnat.plusE;
+  lia.
+- move=> ? -> -> /elem_of_singleton ->; rewrite [tsize (THash _)]tsize_eq; lia.
+- move=> t1 t2 -> _ ->.
+  rewrite tsize_TExpN /= -ssrnat.plusE /=.
+  move/(ssrbool.elimT ssrnat.leP): (tsize_gt0 t1) => ?.
+  move/(ssrbool.elimT ssrnat.leP): (tsize_gt0 t2) => ?.
+  by move=> /elem_of_union [] /elem_of_singleton ->; lia.
+Qed.
+
+Fixpoint public_aux n t : iProp :=
+  if n is S n then
+    minted t ∧ (
+     (∃ T, ⌜decompose T t⌝ ∧ [∗ set] t' ∈ T, public_aux n t')
+     ∨ match t with
+       | TNonce a => pnonce a
+       | TKey kt t => wf_key kt t
+       | THash t => wf_hash t
+       | TEnc (TKey Enc k) t =>
+         wf_enc k t ∧ □ (public_aux n (TKey Dec k) → public_aux n t)
+       | TEnc _ t => True
+       | TExpN' _ _ _ => [∗ list] t' ∈ exps t, dh_pred t' t
+       | _ => False
+       end%I
+    )
+  else False.
+
+Global Instance Persistent_public_aux n t : Persistent (public_aux n t).
+Proof.
+elim: n t => [|n IH] /=; first by apply _.
+case; try by move=> *; apply _.
+case; try by move=> *; apply _.
+case; try by move=> *; apply _.
+Qed.
+
+(** [public t] holds when the term [t] can be declared public. *)
+
+Fact public_key : unit. Proof. exact: tt. Qed.
+Definition public : term → iProp :=
+  locked_with public_key (λ t, public_aux (tsize t) t).
+Canonical public_unlock := [unlockable of public].
+
+Global Instance Persistent_public t : Persistent (public t).
+Proof. rewrite unlock; apply _. Qed.
+
+Lemma public_aux_eq n t : tsize t ≤ n → public_aux n t ⊣⊢ public t.
+Proof.
+rewrite unlock.
+elim: n / (lt_wf n) t => - [|n] _ IH t t_n /=;
+move: (ssrbool.elimT ssrnat.ltP (tsize_gt0 t)) => ?;
+first lia.
+case e_st: (tsize t) => [|m] /=; first lia.
+apply: bi.and_proper => //.
+apply: bi.or_proper.
+- apply: bi.exist_proper => T.
+  apply: and_proper_L => T_t.
+  apply: big_sepS_proper => t' T_t'.
+  move: (decompose_tsize T_t T_t') => ?.
+  rewrite (IH n) ?(IH m) //; lia.
+- case: (t) t_n e_st => //= k.
+  case: k => //= - [] //= k t'.
+  rewrite tsize_eq (tsize_eq (TKey Enc k)) -ssrnat.plusE => t_n e_st.
+  apply: bi.and_proper => //.
+  rewrite !(IH n) ?(IH m) // ?[tsize (TKey _ _)]tsize_eq /=; try lia.
+Qed.
+
+(* TODO: Merge with public_aux_eq *)
+Lemma public_eq t :
+  public t ⊣⊢
+  minted t ∧ (
+      (∃ T, ⌜decompose T t⌝ ∧ [∗ set] t' ∈ T, public t')
+     ∨ match t with
+       | TNonce a => pnonce a
+       | TKey kt t => wf_key kt t
+       | THash t => wf_hash t
+       | TEnc (TKey Enc k) t => wf_enc k t ∧ □ (public (TKey Dec k) → public t)
+       | TEnc _ t => True
+       | TExpN' _ _ _ => [∗ list] t' ∈ exps t, dh_pred t' t
+       | _ => False
+       end%I
+  ).
+Proof.
+rewrite {1}[public]unlock.
+case e_st: (tsize t) => [|m] /=.
+  move: (ssrbool.elimT ssrnat.ltP (tsize_gt0 t)) => ?; lia.
+apply: bi.and_proper => //.
+apply: bi.or_proper.
+- apply: bi.exist_proper => T.
+  apply: and_proper_L => T_t.
+  apply: big_sepS_proper => t' T_t'.
+  move: (decompose_tsize T_t T_t') => ?.
+  rewrite public_aux_eq //; lia.
+- case: (t) e_st => //= k t' e_st.
+  rewrite tsize_eq -ssrnat.plusE in e_st.
+  case: k => // kt k in e_st *.
+  rewrite (tsize_eq (TKey _ _)) in e_st.
+  case: kt => //.
+  apply: bi.and_proper => //.
+  rewrite !public_aux_eq  ?[tsize (TKey _ _)]tsize_eq //=; lia.
+Qed.
+
+Lemma public_minted t : public t ⊢ minted t.
+Proof. rewrite public_eq; by iIntros "[??]". Qed.
+
+Lemma public_TInt n : public (TInt n) ⊣⊢ True.
+Proof.
+apply: (anti_symm _); iIntros "_" => //.
+rewrite public_eq minted_TInt; iSplit => //.
+iLeft; iExists ∅; rewrite big_sepS_empty; iSplit => //.
+by iPureIntro; econstructor.
+Qed.
+
+Lemma public_TPair t1 t2 : public (TPair t1 t2) ⊣⊢ public t1 ∧ public t2.
+Proof.
+apply: (anti_symm _); iIntros "#Ht" => //.
+- rewrite public_eq minted_TPair.
+  iDestruct "Ht" as "([Ht1 Ht2] & publ)".
+  iDestruct "publ" as "[publ | publ]" => //=.
+  iDestruct "publ" as (T) "[%dec publ]".
+  case: dec => //= {}t1 {}t2 -> [-> ->].
+  by rewrite big_sepS_union_pers !big_sepS_singleton.
+- iDestruct "Ht" as "[Ht1 Ht2]".
+  rewrite [public (TPair t1 t2)]public_eq minted_TPair -!public_minted.
+  iSplit; eauto.
+  iLeft; iExists _; iSplit.
+    iPureIntro; by econstructor.
+  by rewrite big_sepS_union_pers !big_sepS_singleton; eauto.
+Qed.
+
+Lemma public_TNonce a :
+  public (TNonce a) ⊣⊢ pnonce a ∗ meta a (nroot.@"minted") ().
+Proof.
+apply: (anti_symm _); iIntros "Ht".
+- rewrite public_eq; iDestruct "Ht" as "[? Ht]".
+  rewrite minted_TNonce. iFrame.
+  iDestruct "Ht" as "[publ | ?]" => //.
+  iDestruct "publ" as (T) "[%dec _]".
+  by case: dec.
+- rewrite public_eq minted_TNonce /pnonce.
+  iDestruct "Ht" as "[Ht ?]". iFrame.
+Qed.
+
+Lemma public_TKey kt t :
+  public (TKey kt t) ⊣⊢ public t ∨ minted t ∧ wf_key kt t.
+Proof.
+apply: (anti_symm _).
+- rewrite public_eq minted_TKey; iDestruct 1 as "[Ht publ]".
+  iDestruct "publ" as "[publ | publ]" => //.
+  + iDestruct "publ" as (T) "[%dec publ]".
+    case: dec => //= {}kt {}t -> [-> ->].
+    by rewrite big_sepS_singleton; eauto.
+  + by eauto.
+- iDestruct 1 as "# [publ | [s_t publ]]".
+    rewrite [public (TKey _ _)]public_eq minted_TKey -public_minted.
+    iSplit => //; iLeft.
+    iExists {[t]}; iSplit; first by iPureIntro; econstructor.
+    by rewrite big_sepS_singleton.
+  rewrite public_eq; iSplit; eauto.
+  by rewrite minted_TKey.
+Qed.
+
+Lemma public_TEnc k t :
+  public (TEnc k t) ⊣⊢
+  public k ∧ public t ∨
+  minted (TEnc k t) ∧
+  match k with
+  | TKey Enc k' => wf_enc k' t ∧ □ (public (TKey Dec k') → public t)
+  | _ => True
+  end.
+Proof.
+apply: (anti_symm _).
+- rewrite public_eq minted_TEnc.
+  iDestruct 1 as "[[Hk Ht] publ]".
+  iDestruct "publ" as "[publ | publ]".
+  + iDestruct "publ" as (T) "[%dec ?]".
+    case: dec => // {}k {}t -> [-> ->].
+    by rewrite big_sepS_union_pers !big_sepS_singleton; iLeft.
+  + iRight. iSplit; first by eauto.
+    case: k => // - [] k; eauto.
+- iDestruct 1 as "[#[Hk Ht] | (#Ht & inv)]".
+  { rewrite [public (TEnc _ _)]public_eq minted_TEnc.
+    rewrite -!public_minted.
+    iSplit; eauto; iLeft.
+    iExists {[k; t]}; rewrite big_sepS_union_pers !big_sepS_singleton.
+    iSplit; eauto; iPureIntro; by econstructor. }
+  rewrite [public (TEnc _ _)]public_eq; iSplit => //. by eauto.
+Qed.
+
+Lemma public_THash t :
+  public (THash t) ⊣⊢ public t ∨ minted t ∧ wf_hash t.
+Proof.
+apply: (anti_symm _).
+- rewrite public_eq minted_THash.
+  iDestruct 1 as "[Ht [publ | publ]]" => //; eauto.
+  iDestruct "publ" as (T) "[%dec ?]".
+  case: dec => //= {}t -> [->].
+  by rewrite big_sepS_singleton; eauto.
+- iDestruct 1 as "[Ht | [? publ]]".
+    rewrite [public (THash _)]public_eq minted_THash -public_minted.
+    iSplit => //=; iLeft.
+    iExists {[t]}; rewrite big_sepS_singleton; iSplit => //.
+    iPureIntro; by econstructor.
+  rewrite public_eq; iSplit.
+    by rewrite minted_THash.
+  by eauto.
+Qed.
+
+(* MOVE *)
+Lemma exps_TExpN t ts : exps (TExpN t ts) ≡ₚ exps t ++ ts.
+Proof.
+apply/(ssrbool.elimT perm_Perm).
+rewrite exps_TExpN.
+by rewrite path.perm_sort seq.perm_cat2l.
+Qed.
+
+Lemma eq_op_bool_decide
+  {T : eqtype.Equality.type}
+  {_ : EqDecision (eqtype.Equality.sort T)}
+  (x y : eqtype.Equality.sort T) :
+  bool_decide (x = y) = (eqtype.eq_op x y).
+Proof.
+apply/(ssrbool.sameP).
+- exact: bool_decide_reflect.
+- exact: eqtype.eqP.
+Qed.
+
+Lemma is_exp_TExpN t ts :
+  is_exp (TExpN t ts) = implb (bool_decide (ts = [])) (is_exp t).
+Proof.
+rewrite is_exp_TExpN -eq_op_bool_decide implb_orb.
+by case: ts.
+Qed.
+
+Lemma base_exps_inj t1 t2 :
+  base t1 = base t2 →
+  exps t1 ≡ₚ exps t2 →
+  t1 = t2.
+Proof.
+move=> eb /(ssrbool.introT perm_Perm) ?.
+by apply: base_exps_inj.
+Qed.
+
+Lemma TExp_TExpN t1 ts1 t2 : TExp (TExpN t1 ts1) t2 = TExpN t1 (t2 :: ts1).
+Proof.
+by rewrite TExpNA -[@seq.cat]/@app [_ ++ _]comm.
+Qed.
+
+Lemma base_expN t : ¬ is_exp t → base t = t.
+Proof.
+move=> tNX; apply: base_expN.
+apply/(ssrbool.introN ssrbool.idP).
+by rewrite is_trueP.
+Qed.
+
+Lemma exps_expN t : ¬ is_exp t → exps t = [].
+Proof.
+move=> tNX; apply: exps_expN.
+apply/(ssrbool.introN ssrbool.idP).
+by rewrite is_trueP.
+Qed.
+
+Lemma TExp0 t : TExpN t [] = t.
+Proof.
+apply: base_exps_inj; first by rewrite base_TExpN.
+by rewrite exps_TExpN app_nil_r.
+Qed.
+
+Lemma is_exp_base t : ¬ is_exp (base t).
+Proof.
+rewrite (ssrbool.negbTE (is_exp_base t)) /=. by auto.
+Qed.
+Hint Resolve is_exp_base : core.
+(* /MOVE *)
+
+Lemma public_TExpN t ts :
+  ¬ is_exp t →
+  ts ≠ [] →
+  public (TExpN t ts) ⊣⊢
+  (∃ t' ts', ⌜ts ≡ₚ t' :: ts'⌝ ∧ public (TExpN t ts') ∧ public t') ∨
+  minted (TExpN t ts) ∧ [∗ list] t' ∈ ts, dh_pred t' (TExpN t ts).
+Proof.
+move=> tNX tsN0.
+have ttsX : is_exp (TExpN t ts).
+  by rewrite is_exp_TExpN; case: (ts) tsN0.
+have [? [] ? [] H etts] : ∃ t' ts' H, TExpN t ts = TExpN' t' ts' H.
+  case: (TExpN t ts) ttsX => //=; eauto.
+apply: (anti_symm _).
+- rewrite public_eq minted_TExpN {2}etts {H etts}.
+  iDestruct 1 as "[# [Ht Hts] [#publ | #publ]]".
+  + iDestruct "publ" as (T) "[%dec publ]".
+    move e: (TExpN t ts) => t' in dec ttsX *.
+    case: dec ttsX; try by move=> * {e}; subst t'.
+    rewrite -{}e {t'}.
+    move=> t1 t2 -> _ e _.
+    rewrite big_sepS_union_pers !big_sepS_singleton.
+    iDestruct "publ" as "[publ1 publ2]".
+    iLeft. iExists t2, (exps t1).
+    have -> : TExpN t (exps t1) = t1.
+      apply: base_exps_inj.
+      * by move/(f_equal base): e; rewrite !base_TExpN.
+      * by rewrite exps_TExpN exps_expN //=.
+    do !iSplit => //. iPureIntro.
+    have ->: ts ≡ₚ exps (TExpN t ts).
+      by rewrite exps_TExpN exps_expN //; apply/is_trueP.
+    by rewrite e exps_TExpN [_ ++ _]comm.
+  + iRight; do 2?iSplit => //.
+    by rewrite exps_TExpN exps_expN.
+- iDestruct 1 as "# [publ | publ]".
+  + iDestruct "publ" as (t' ts') "[%e [Ht1 Ht2]]".
+    rewrite e in ttsX *.
+    rewrite [public (TExpN _ (_ :: _))]public_eq minted_TExpN /=.
+    iSplit.
+      rewrite !public_minted minted_TExpN /=.
+      by iDestruct "Ht1" as "[??]"; eauto.
+    iLeft.
+    iExists {[TExpN t ts'; t']}.
+    rewrite big_sepS_union_pers !big_sepS_singleton.
+    do !iSplit => //.
+    iPureIntro.
+    rewrite -TExp_TExpN; apply: DExp; eauto.
+    by rewrite TExp_TExpN.
+  + iDestruct "publ" as "[s p]"; rewrite public_eq [minted]unlock; iSplit=> //.
+    rewrite {4}etts; iRight.
+    by rewrite exps_TExpN exps_expN //.
+Qed.
+
+Lemma public_TExp_iff t1 t2 :
+  ¬ is_exp t1 →
+  public (TExp t1 t2) ⊣⊢
+  public t1 ∧ public t2 ∨
+  minted t1 ∧ minted t2 ∧ dh_pred t2 (TExp t1 t2).
+Proof.
+move=> ?; rewrite public_TExpN //=.
+apply: (anti_symm _); iIntros "#pub".
+- iDestruct "pub" as "[pub | pub]" => //.
+    iDestruct "pub" as (??) "(%e & p_t1 & p_t2)".
+    symmetry in e.
+    case/Permutation_singleton_r: e => -> ->; eauto.
+    rewrite TExp0; eauto.
+  by rewrite minted_TExp /=; iDestruct "pub" as "[[??] [??]]"; eauto.
+- iDestruct "pub" as "[[p1 p2] | (s1 & s2 & pub)]".
+    by iLeft; iExists t2, []; rewrite TExp0; eauto.
+  by iRight; rewrite /= minted_TExp; do !iSplit => //=.
+Qed.
+
+Lemma public_TExp2_iff t1 t2 t3 :
+  ¬ is_exp t1 →
+  public (TExpN t1 [t2; t3]) ⊣⊢
+  public (TExpN t1 [t2]) ∧ public t3 ∨
+  public (TExpN t1 [t3]) ∧ public t2 ∨
+  minted (TExpN t1 [t2; t3]) ∧
+  dh_pred t2 (TExpN t1 [t2; t3]) ∧
+  dh_pred t3 (TExpN t1 [t2; t3]).
+Proof.
+move=> t1NX. rewrite public_TExpN //.
+apply: (anti_symm _); iIntros "#pub".
+- rewrite /=; iDestruct "pub" as "[pub | (? & ? & ? & _)]" => //; eauto.
+  iDestruct "pub" as (??) "(%e & p_t1 & p_t2)".
+  by case: (Permutation_length_2_inv e) => [[-> ->] | [-> ->]]; eauto.
+- iDestruct "pub" as "[[? ?] | [[? ?] | (? & ? & ?)]]".
+  + iLeft; iExists t3, [t2]; do !iSplit => //.
+    iPureIntro; apply: perm_swap.
+  + by iLeft; iExists t2, [t3]; do !iSplit => //.
+  + iRight; do !iSplit => //=.
+Qed.
+
+Lemma public_TExp t1 t2 :
+  public t1 -∗
+  public t2 -∗
+  public (TExp t1 t2).
+Proof.
+iIntros "#p1 #p2".
+rewrite -{2}(base_expsK t1) TExp_TExpN public_TExpN //.
+by iLeft; iExists t2, (exps t1); rewrite base_expsK; eauto.
+Qed.
+
+Lemma public_to_list t ts :
+  Spec.to_list t = Some ts →
+  public t -∗ [∗ list] t' ∈ ts, public t'.
+Proof.
+elim/term_ind': t ts => //=.
+  by case=> // ts [<-] /=; iIntros "?".
+move=> t _ tl IH ts.
+case e: (Spec.to_list tl) => [ts'|] // [<-] /=.
+rewrite public_TPair /=; iIntros "[??]"; iFrame.
+by iApply IH.
+Qed.
+
+Lemma public_of_list ts :
+  public (Spec.of_list ts) ⊣⊢
+  [∗ list] t ∈ ts, public t.
+Proof.
+rewrite Spec.of_list_unseal.
+elim: ts => [|t ts IH]; first by rewrite public_TInt.
+by rewrite public_TPair /= IH bi.persistent_and_sep.
+Qed.
+
+Lemma public_tag N t : public (Spec.tag N t) ⊣⊢ public t.
+Proof.
+by rewrite Spec.tag_unseal public_TPair public_TInt bi.emp_and.
+Qed.
+
+Lemma public_TEncE N Φ k t :
+  public (TEnc (TKey Enc k) (Spec.tag N t)) -∗
+  enc_pred N Φ -∗
+  public (TKey Enc k) ∧ public t ∨
+  □ ▷ Φ k t ∧ minted t ∧ □ (public (TKey Dec k) → public t).
+Proof.
+iIntros "#Ht #HΦ"; rewrite public_TEnc -(public_tag N t).
+iDestruct "Ht" as "[[? Ht] | Ht]"; first by eauto.
+rewrite minted_TEnc minted_tag.
+iDestruct "Ht" as "([??] & inv & ?)".
+iRight; iSplit; eauto; by iApply wf_enc_elim.
+Qed.
+
+Lemma public_TEncI N Φ k t :
+  enc_pred N Φ -∗
+  minted k -∗
+  minted t -∗
+  (∀ k',
+    ⌜k = TKey Enc k'⌝ -∗
+    □ Φ k' t ∗
+    □ (public (TKey Dec k') → public t)) -∗
+  public (TEnc k (Spec.tag N t)).
+Proof.
+iIntros "#HΦ #m_k #m_t Henc".
+rewrite public_TEnc minted_TEnc minted_tag.
+iRight. do !iSplit => //.
+case: k => //; case=> // k.
+iDestruct ("Henc" $! k with "[//]") as "[#H1 #H2]".
+rewrite public_tag; iSplit => //.
+iExists N, t, Φ; eauto.
+Qed.
+
+Lemma public_TEncIS N Φ k t :
+  minted (TKey Enc k) -∗
+  enc_pred N Φ -∗
+  □ Φ k t -∗
+  minted t -∗
+  □ (public (TKey Dec k) → public t) -∗
+  public (TEnc (TKey Enc k) (Spec.tag N t)).
+Proof.
+iIntros "#Henc #HΦ #HΦt #Ht #Hdecl".
+rewrite public_TEnc; iRight.
+rewrite minted_TEnc minted_tag.
+iSplit; first by rewrite minted_TKey; eauto.
+rewrite public_tag. iSplit; eauto.
+iExists N, t, Φ; eauto.
+Qed.
+
+Lemma public_TEncIP k t :
+  public k -∗
+  public t -∗
+  public (TEnc k t).
+Proof. by iIntros "? ?"; rewrite public_TEnc; eauto. Qed.
+
+Lemma nonce_alloc P Q a :
+  meta_token a ⊤ -∗
+  (minted (TNonce a) -∗ False) ∧
+  |==> minted (TNonce a) ∗
+    □ (public (TNonce a) ↔ ▷ □ P (TNonce a)) ∗
+    □ (∀ t, dh_pred (TNonce a) t ↔ ▷ □ Q t).
+Proof.
+iIntros "token".
+iSplit.
+{ rewrite minted_TNonce. iIntros "contra".
+  by iDestruct (meta_meta_token with "token contra") as "[]". }
+iMod (saved_pred_alloc P DfracDiscarded) as (γP) "#own_P" => //.
+iMod (saved_pred_alloc Q DfracDiscarded) as (γQ) "#own_Q" => //.
+rewrite (meta_token_difference a (↑nroot.@"nonce")) //.
+iDestruct "token" as "[nonce token]".
+iMod (meta_set _ _ γP with "nonce") as "#nonce"; eauto.
+rewrite (meta_token_difference a (↑nroot.@"dh")); last solve_ndisj.
+iDestruct "token" as "[dh token]".
+iMod (meta_set _ _ γQ with "dh") as "#dh"; eauto.
+rewrite (meta_token_difference a (↑nroot.@"minted")); last solve_ndisj.
+iDestruct "token" as "[minted token]".
+iMod (meta_set _ _ () (nroot.@"minted") with "minted") as "#minted" => //.
+iSplitR.
+  by rewrite minted_TNonce.
+iSplitR.
+  rewrite public_TNonce; do 2!iModIntro; iSplit.
+  + iIntros "[#public _]".
+    iDestruct "public" as (γP' P') "(#meta_γP' & #own_P' & ?)".
+    iPoseProof (meta_agree with "nonce meta_γP'") as "->".
+    iPoseProof (saved_pred_agree _ _ _ _ _ (TNonce a) with "own_P own_P'") as "e".
+    by iModIntro; iRewrite "e".
+  + iIntros "#?". iSplit => //. iExists γP, P; eauto.
+iIntros "!> !> %t"; iSplit.
+- iDestruct 1 as (γQ' Q') "(#meta_γQ' & #own_Q' & ?)".
+  iPoseProof (meta_agree with "dh meta_γQ'") as "->".
+  iPoseProof (saved_pred_agree _ _ _ _ _ t with "own_Q own_Q'") as "e".
+  by iModIntro; iRewrite "e".
+- by iIntros "#?"; iExists _, _; eauto.
+Qed.
+
+Definition public_ctx : iProp :=
+  key_pred (nroot.@"keys".@"sym") (λ _  _, False%I) ∗
+  key_pred (nroot.@"keys".@"enc") (λ kt _, ⌜kt = Enc⌝)%I ∗
+  key_pred (nroot.@"keys".@"sig") (λ kt _, ⌜kt = Dec⌝)%I.
+
+#[global]
+Instance public_ctx_persistent : Persistent public_ctx.
+Proof. apply _. Qed.
+
+Class HasPublicCtx (ctx : iProp) := {
+  has_public_ctx : ctx ⊢ public_ctx;
+  has_public_ctx_persistent : Persistent ctx;
+}.
+
+Local Existing Instance has_public_ctx_persistent.
+
+Context `{!HasPublicCtx ctx}.
+
+Lemma public_sym_keyE kt k :
+  ctx -∗
+  public (TKey kt (Spec.tag (nroot.@"keys".@"sym") k)) -∗
+  ◇ public k.
+Proof.
+iIntros "ctx #p_k".
+iDestruct (has_public_ctx with "ctx") as "(#sym & _)".
+rewrite public_TKey public_tag. iDestruct "p_k" as "[p_k|[_ p_k]]"; eauto.
+by iDestruct (wf_key_elim with "[//] [//]") as "#>[]".
+Qed.
+
+Lemma public_sym_key kt k :
+  ctx -∗
+  public (TKey kt (Spec.tag (nroot.@"keys".@"sym") k)) ↔
+  minted k ∧ ◇ public k.
+Proof.
+iIntros "ctx".
+iDestruct (has_public_ctx with "ctx") as "(#sym & _)".
+rewrite public_TKey !public_tag minted_tag.
+iSplit.
+- iIntros "[#p_k|[#m_k #wf]]"; eauto.
+  + iSplit => //. by iApply public_minted.
+  + iSplit => //. by iDestruct (wf_key_elim with "[//] [//]") as "#>%".
+- rewrite /bi_except_0. iIntros "[#m_k [#fail|#p_k]]".
+  + iRight; iSplit => //.
+    by iExists _, _, _; iSplit => //; iSplit => //.
+  + by iLeft.
+Qed.
+
+Lemma public_enc_key kt k :
+  ctx -∗
+  public (TKey kt (Spec.tag (nroot.@"keys".@"enc") k)) ↔
+  minted k ∧ ◇ (⌜kt = Enc⌝ ∨ public k).
+Proof.
+iIntros "ctx".
+iDestruct (has_public_ctx with "ctx") as "(_ & #enc & _)".
+rewrite public_TKey !public_tag minted_tag.
+iSplit.
+- iIntros "[#p_k|[#m_k #wf]]"; eauto.
+  + iSplit; eauto. by iApply public_minted.
+  + iSplit => //.
+    iDestruct (wf_key_elim with "[//] [//]") as "#>%".
+    by eauto.
+- rewrite /bi_except_0. iIntros "[#m_k [#fail|[->|#p_k]]]".
+  + iRight; iSplit => //.
+    iExists _, _, _; iSplit => //; iSplit => //.
+    iIntros "!> !>". by iDestruct "fail" as "[]".
+  + iRight. iSplit => //.
+    by iExists _, _, _; eauto.
+  + by iLeft.
+Qed.
+
+Lemma public_sig_key kt k :
+  ctx -∗
+  public (TKey kt (Spec.tag (nroot.@"keys".@"sig") k)) ↔
+  minted k ∧ ◇ (⌜kt = Dec⌝ ∨ public k).
+Proof.
+iIntros "ctx".
+iDestruct (has_public_ctx with "ctx") as "(_ & _ & #sig)".
+rewrite public_TKey !public_tag minted_tag.
+iSplit.
+- iIntros "[#p_k|[#m_k #wf]]"; eauto.
+  + iSplit; eauto. by iApply public_minted.
+  + iSplit => //.
+    iDestruct (wf_key_elim with "[//] [//]") as "#>%".
+    by eauto.
+- rewrite /bi_except_0. iIntros "[#m_k [#fail|[->|#p_k]]]".
+  + iRight; iSplit => //.
+    iExists _, _, _; iSplit => //; iSplit => //.
+    iIntros "!> !>". by iDestruct "fail" as "[]".
+  + iRight. iSplit => //.
+    by iExists _, _, _; eauto.
+  + by iLeft.
+Qed.
+
+Lemma public_mkskey k :
+  ctx -∗
+  public (Spec.mkskey k) ↔ minted k ∧ ◇ public k.
+Proof.
+iIntros "#ctx".
+iDestruct (has_public_ctx with "ctx") as "#(sym & _)".
+rewrite public_TPair. iSplit.
+- iIntros "[#p_k _]".
+  by iApply (public_sym_key with "[//] p_k").
+- by iIntros "#?"; iSplit; iApply (public_sym_key with "[//]").
+Qed.
+
+Lemma public_enc_keyE k :
+  ctx -∗
+  public (TKey Dec (Spec.tag (nroot.@"keys".@"enc") k)) -∗
+  ◇ public k.
+Proof.
+iIntros "#ctx #p_k".
+iDestruct (has_public_ctx with "ctx") as "#(_ & enc & _)".
+rewrite public_TKey public_tag. iDestruct "p_k" as "[p_k|[_ p_k]]"; eauto.
+by iDestruct (wf_key_elim with "[//] [//]") as "#>%".
+Qed.
+
+Lemma public_sig_keyE k :
+  ctx -∗
+  public (TKey Enc (Spec.tag (nroot.@"keys".@"sig") k)) -∗
+  ◇ public k.
+Proof.
+iIntros "#ctx #p_k".
+iDestruct (has_public_ctx with "ctx") as "#(_ & _ & sig)".
+rewrite public_TKey public_tag. iDestruct "p_k" as "[p_k|[_ p_k]]"; eauto.
+by iDestruct (wf_key_elim with "[//] [//]") as "#>%".
+Qed.
+
+End Public.
+
+Arguments public_enc_name {Σ _}.
+Arguments enc_pred {Σ _} N Φ.
+Arguments enc_pred_set {Σ _ _} N Φ.
+Arguments enc_pred_token_difference {Σ _} E1 E2.
+Arguments public_hash_name {Σ _}.
+Arguments hash_pred {Σ _} N P.
+Arguments hash_pred_set {Σ _ _} N P.
+Arguments hash_pred_token_difference {Σ _} E1 E2.
+Arguments public_key_name {Σ _}.
+Arguments key_pred {Σ _} N φ.
+Arguments key_pred_set {Σ _ _} N P.
+Arguments key_pred_token_difference {Σ _} E1 E2.
+
+Lemma publicGS_alloc `{!heapGS Σ} E :
+  publicGpreS Σ →
+  ⊢ |={E}=> ∃ (H : publicGS Σ),
+             public_ctx ∗
+             enc_pred_token ⊤ ∗
+             key_pred_token (⊤ ∖ ↑nroot.@"keys") ∗
+             hash_pred_token ⊤.
+Proof.
+move=> ?; iStartProof.
+iMod (own_alloc (reservation_map_token ⊤)) as (γ_enc) "own_enc".
+  apply reservation_map_token_valid.
+iMod (own_alloc (reservation_map_token ⊤)) as (γ_key) "own_key".
+  apply reservation_map_token_valid.
+iMod (own_alloc (reservation_map_token ⊤)) as (γ_hash) "own_hash".
+  apply reservation_map_token_valid.
+pose (H := PublicGS _ γ_enc γ_key γ_hash).
+iExists H. iFrame.
+iAssert (key_pred_token ⊤) with "[own_enc]" as "token".
+  by iFrame.
+rewrite (key_pred_token_difference (↑nroot.@"keys")) //.
+iDestruct "token" as "[token ?]"; iFrame.
+iMod (key_pred_set (nroot.@"keys".@"sym") (λ _ _, False%I) with "token")
+    as "[#? token]"; try solve_ndisj.
+iMod (key_pred_set (nroot.@"keys".@"enc") (λ kt _, ⌜kt = Enc⌝)%I with "token")
+    as "[#? token]"; try solve_ndisj.
+iMod (key_pred_set (nroot.@"keys".@"sig") (λ kt _, ⌜kt = Dec⌝)%I with "token")
+    as "[#? token]"; try solve_ndisj.
+iModIntro. rewrite /public_ctx. eauto.
+Qed.
