core/term.v
@@ -5,7 +5,7 @@ From stdpp Require Import gmap.
 From iris.heap_lang Require Import notation.
 From iris.heap_lang Require Import primitive_laws.
 From cryptis Require Import mathcomp_compat lib.
-From cryptis Require Export pre_term.
+From cryptis.core Require Export pre_term.
 
 Definition int_of_key_type kt : Z :=
   match kt with
