core/term_meta.v
@@ -1,0 +1,400 @@
+From mathcomp Require Import ssreflect.
+From stdpp Require Import gmap.
+From iris.algebra Require Import agree auth gset gmap list reservation_map excl.
+From iris.algebra Require Import functions.
+From iris.base_logic.lib Require Import saved_prop invariants.
+From iris.heap_lang Require Import notation proofmode.
+From cryptis Require Import lib gmeta nown.
+From cryptis.core Require Import term comp_map minted.
+
+Set Implicit Arguments.
+Unset Strict Implicit.
+Unset Printing Implicit Defensive.
+
+Definition term_namesUR := authUR (gmapUR term (agreeR gnameO)).
+
+Class term_metaGpreS Σ : Type := TermMetaGPreS {
+  term_meta_meta : metaGS Σ;
+  term_meta_names : inG Σ term_namesUR;
+}.
+
+Local Existing Instance term_meta_meta.
+Local Existing Instance term_meta_names.
+
+Class term_metaGS Σ : Type := TermMetaGS {
+  term_meta_inG  : term_metaGpreS Σ;
+  term_meta_name : gname;
+}.
+
+Global Existing Instance term_meta_inG.
+
+Definition term_metaΣ : gFunctors :=
+  #[metaΣ; GFunctor term_namesUR].
+
+Global Instance subG_term_metaGpreS Σ :
+  subG term_metaΣ Σ → term_metaGpreS Σ.
+Proof. solve_inG. Qed.
+
+Section TermMeta.
+
+Context `{!heapGS Σ}.
+Notation iProp := (iProp Σ).
+Notation iPropO := (iPropO Σ).
+Notation iPropI := (iPropI Σ).
+
+Definition term_meta_inv `{!term_metaGS Σ} : iProp :=
+  ∃ names : gmap term gname,
+    own term_meta_name (● ((to_agree <$> names) : gmap _ _)) ∗
+    [∗ set] t ∈ dom names, minted t.
+
+Definition term_meta_ctx `{!term_metaGS Σ} : iProp :=
+  inv (nroot.@"cryptis".@"meta") term_meta_inv.
+
+Lemma term_metaGS_alloc E :
+  term_metaGpreS Σ →
+  ⊢ |={E}=> ∃ (H : term_metaGS Σ), term_meta_ctx.
+Proof.
+move=> ?; iStartProof.
+iMod (own_alloc (● (∅ : gmap term (agree gname)))) as (γ_names) "names_auth".
+  by apply auth_auth_valid.
+pose (H := TermMetaGS _ γ_names).
+iExists H. iApply inv_alloc.
+iExists ∅. rewrite fmap_empty /=. iFrame.
+by rewrite dom_empty_L big_sepS_empty.
+Qed.
+
+Context `{!term_metaGS Σ}.
+
+Global Instance term_meta_inv_timeless : Timeless term_meta_inv.
+Proof. rewrite /term_meta_inv. apply _. Qed.
+
+#[global]
+Instance term_meta_ctx_persistent : Persistent term_meta_ctx.
+Proof. apply _. Qed.
+
+Class HasTermMetaCtx (ctx : iProp) := {
+  has_term_meta_ctx : ctx ⊢ term_meta_ctx;
+  has_term_meta_ctx_persistent : Persistent ctx;
+}.
+
+Local Existing Instance has_term_meta_ctx_persistent.
+
+Context `{!HasTermMetaCtx ctx}.
+
+Definition term_name t γ : iProp :=
+  own term_meta_name (◯ {[t := to_agree γ]}).
+
+Global Instance term_name_persistent t γ : Persistent (term_name t γ).
+Proof. apply _. Qed.
+
+Global Instance term_name_timeless t γ : Timeless (term_name t γ).
+Proof. apply _. Qed.
+
+Lemma term_name_agree t γ1 γ2 :
+  term_name t γ1 -∗
+  term_name t γ2 -∗
+  ⌜γ1 = γ2⌝.
+Proof.
+iIntros "name1 name2".
+iPoseProof (own_valid_2 with "name1 name2") as "%valid".
+rewrite -auth_frag_op auth_frag_valid in valid.
+move/(_ t): valid.
+rewrite lookup_op !lookup_singleton -Some_op Some_valid.
+by move=> /to_agree_op_inv_L ->.
+Qed.
+
+Definition term_token_def t E : iProp :=
+  ∃ γ, term_name t γ ∗ gmeta_token γ E.
+Definition term_token_aux : seal term_token_def. by eexists. Qed.
+Definition term_token := unseal term_token_aux.
+Lemma term_token_unseal : term_token = term_token_def.
+Proof. exact: seal_eq. Qed.
+
+Definition term_meta_def `{Countable L} t N (x : L) : iProp :=
+  ∃ γ, term_name t γ ∗ gmeta γ N x.
+Definition term_meta_aux : seal (@term_meta_def). by eexists. Qed.
+Definition term_meta := unseal term_meta_aux.
+Lemma term_meta_unseal : @term_meta = @term_meta_def.
+Proof. exact: seal_eq. Qed.
+Arguments term_meta {L _ _} t N x.
+
+Global Instance term_token_timeless t E : Timeless (term_token t E).
+Proof. rewrite term_token_unseal. apply _. Qed.
+
+Global Instance term_meta_timeless `{Countable L} t N (x : L) :
+  Timeless (term_meta t N x).
+Proof. rewrite term_meta_unseal. apply _. Qed.
+
+Global Instance term_meta_persistent `{Countable L} t N (x : L) :
+  Persistent (term_meta t N x).
+Proof. rewrite term_meta_unseal. apply _. Qed.
+
+Lemma term_token_drop E1 E2 t :
+  E1 ⊆ E2 → term_token t E2 -∗ term_token t E1.
+Proof.
+rewrite term_token_unseal.
+iIntros "% (%γ & #name & token)".
+iExists γ. iSplit => //. by iApply gmeta_token_drop.
+Qed.
+
+Lemma term_token_disj E1 E2 t :
+  term_token t E1 -∗ term_token t E2 -∗ ⌜E1 ## E2⌝.
+Proof.
+rewrite term_token_unseal.
+iIntros "(% & #name1 & token1) (% & #name2 & token2)".
+iPoseProof (term_name_agree with "name1 name2") as "<-".
+iApply (gmeta_token_disj with "token1 token2").
+Qed.
+
+Lemma term_token_difference t E1 E2 :
+  E1 ⊆ E2 → term_token t E2 ⊣⊢ term_token t E1 ∗ term_token t (E2 ∖ E1).
+Proof.
+rewrite term_token_unseal.
+move=> sub. iSplit.
+- iIntros "(% & #name & token)".
+  rewrite (gmeta_token_difference _ _ _ sub).
+  iDestruct "token" as "[token1 token2]".
+  by iSplitL "token1"; iExists _; iFrame.
+- iIntros "[(% & #name1 & token1) (% & #name2 & token2)]".
+  iPoseProof (term_name_agree with "name1 name2") as "<-".
+  iExists _; iSplit => //.
+  rewrite (gmeta_token_difference _ _ _ sub). by iFrame.
+Qed.
+
+Lemma term_meta_token `{Countable L} t (x : L) N E :
+  ↑N ⊆ E → term_token t E -∗ term_meta t N x -∗ False.
+Proof.
+rewrite term_token_unseal term_meta_unseal => sub.
+iIntros "(% & #name1 & token) (% & #name2 & #meta)".
+iPoseProof (term_name_agree with "name1 name2") as "<-".
+by iApply (gmeta_gmeta_token with "token meta").
+Qed.
+
+Lemma term_meta_set' `{Countable L} N (x : L) E t :
+  ↑N ⊆ E → term_token t E ==∗ term_meta t N x ∗ term_token t (E ∖ ↑N).
+Proof.
+rewrite term_token_unseal term_meta_unseal.
+iIntros "%sub (%γ & #name & token)".
+iMod (gmeta_set' _ _ _ x sub with "token") as "[#meta token]".
+iModIntro.
+by iSplit; iExists _; iSplit => //.
+Qed.
+
+Lemma term_meta_set `{Countable L} N (x : L) E t :
+  ↑N ⊆ E → term_token t E ==∗ term_meta t N x.
+Proof.
+iIntros "%sub token".
+iMod (term_meta_set' x _ sub with "token") as "[#meta token]".
+by iModIntro.
+Qed.
+
+Lemma term_meta_agree `{Countable L} t N (x1 x2 : L) :
+  term_meta t N x1 -∗ term_meta t N x2 -∗ ⌜x1 = x2⌝.
+Proof.
+rewrite term_meta_unseal.
+iIntros "(% & #name1 & #meta1) (% & #name2 & #meta2)".
+iPoseProof (term_name_agree with "name1 name2") as "<-".
+iApply (gmeta_agree with "meta1 meta2").
+Qed.
+
+Lemma term_token_switch t N' Q : ⊢ switch (term_token t (↑N')) Q.
+Proof.
+iExists (term_meta t N' ()). iSplit; iModIntro.
+- iIntros "[token #meta]".
+  by iDestruct (term_meta_token with "token meta") as "[]".
+- iIntros "token".
+  by iMod (term_meta_set () with "token") as "#meta".
+Qed.
+
+Section TermOwn.
+
+Definition term_own_def `{inG Σ A} t N (x : A) : iProp :=
+  ∃ γ, term_name t γ ∗ nown γ N x.
+Definition term_own_aux : seal (@term_own_def). by eexists. Qed.
+Definition term_own := unseal (@term_own_aux).
+Lemma term_own_unseal : @term_own = @term_own_def.
+Proof. exact: seal_eq. Qed.
+Arguments term_own {A _} t N x.
+
+Context `{inG Σ A}.
+
+Lemma term_own_alloc t N {E} (a : A) :
+  ↑N ⊆ E → ✓ a → term_token t E ==∗ term_own t N a ∗ term_token t (E ∖ ↑N).
+Proof.
+rewrite term_own_unseal term_token_unseal.
+iIntros "%sub %val (% & #name & token)".
+iMod (nown_alloc _ _ sub val with "token") as "[own token]".
+iModIntro.
+by iSplitL "own"; iExists _; iFrame.
+Qed.
+
+Lemma term_own_valid t N (a : A) : term_own t N a -∗ ✓ a.
+Proof.
+rewrite term_own_unseal.
+iIntros "(%γ' & #own_γ & own)". iApply (nown_valid with "own").
+Qed.
+
+Lemma term_own_valid_2 t N (a1 a2 : A) :
+  term_own t N a1 -∗ term_own t N a2 -∗ ✓ (a1 ⋅ a2).
+Proof.
+rewrite term_own_unseal.
+iIntros "(%γ1 & #own_γ1 & own1) (%γ2 & #own_γ2 & own2)".
+iPoseProof (term_name_agree with "own_γ1 own_γ2") as "<-".
+by iApply (nown_valid_2 with "own1 own2").
+Qed.
+
+Lemma term_own_update t N (a a' : A) :
+  a ~~> a' → term_own t N a ==∗ term_own t N a'.
+Proof.
+rewrite term_own_unseal.
+iIntros (?) "(%γ' & #? & own)".
+iMod (nown_update with "own") as "own"; eauto.
+iModIntro. iExists γ'. eauto.
+Qed.
+
+#[global]
+Instance term_own_core_persistent t N (a : A) :
+  CoreId a → Persistent (term_own t N a).
+Proof. rewrite term_own_unseal. apply _. Qed.
+
+#[global]
+Instance term_own_timeless t N (a : A) :
+  Discrete a → Timeless (term_own t N a).
+Proof. rewrite term_own_unseal. apply _. Qed.
+
+#[global]
+Instance term_own_ne t N : NonExpansive (@term_own A _ t N).
+Proof. rewrite term_own_unseal. solve_proper. Qed.
+
+#[global]
+Instance term_own_proper t N : Proper ((≡) ==> (≡)) (@term_own A _ t N).
+Proof. rewrite term_own_unseal. solve_proper. Qed.
+
+Lemma term_own_op t N (a1 a2 : A) :
+  term_own t N (a1 ⋅ a2) ⊣⊢ term_own t N a1 ∗ term_own t N a2.
+Proof.
+rewrite term_own_unseal.
+iSplit.
+- iIntros "(%γ' & #? & [own1 own2])".
+  by iSplitL "own1"; iExists γ'; iSplit.
+- iIntros "[(%γ1 & #own_γ1 & own1) (%γ2 & #own_γ2 & own2)]".
+  iPoseProof (term_name_agree with "own_γ1 own_γ2") as "<-".
+  iExists γ1. iSplit => //. by iSplitL "own1".
+Qed.
+
+#[global]
+Instance from_sep_term_own t N (a b1 b2 : A) :
+  IsOp a b1 b2 → FromSep (term_own t N a) (term_own t N b1) (term_own t N b2).
+Proof.
+by rewrite /IsOp /FromSep => ->; rewrite term_own_op.
+Qed.
+
+#[global]
+Instance combine_sep_as_term_own t N (a b1 b2 : A) :
+  IsOp a b1 b2 → CombineSepAs (term_own t N b1) (term_own t N b2) (term_own t N a).
+Proof. exact: from_sep_term_own. Qed.
+
+#[global]
+Instance into_sep_term_own t N (a b1 b2 : A) :
+  IsOp a b1 b2 → IntoSep (term_own t N a) (term_own t N b1) (term_own t N b2).
+Proof.
+by rewrite /IsOp /IntoSep => ->; rewrite term_own_op.
+Qed.
+
+Lemma term_own_mono t N (a1 a2 : A) : a1 ≼ a2 → term_own t N a2 -∗ term_own t N a1.
+Proof.
+case => ? ->.
+rewrite term_own_op.
+by iIntros "[??]".
+Qed.
+
+Lemma term_own_update_2 t N (a1 a2 a' : A) :
+  a1 ⋅ a2 ~~> a' →
+  term_own t N a1 -∗
+  term_own t N a2 ==∗
+  term_own t N a'.
+Proof.
+iIntros "% H1 H2".
+iMod (term_own_update with "[H1 H2]") as "H" => //.
+by iSplitL "H1".
+Qed.
+
+End TermOwn.
+
+#[global] Typeclasses Opaque term_own.
+
+Lemma term_token_alloc_aux (T : gset term) (P Q : iProp) E :
+  (∀ t, ⌜t ∈ T⌝ -∗ P -∗ minted t -∗ False) -∗
+  (∀ t, ⌜t ∈ T⌝ -∗ Q -∗ minted t) -∗
+  (P ∧ |={E}=> Q) -∗
+  term_meta_inv ={E}=∗
+  term_meta_inv ∗ Q ∗ [∗ set] t ∈ T, term_token t ⊤.
+Proof.
+assert (∀ names : gmap term gname,
+  dom names ## T →
+  own term_meta_name (● ((to_agree <$> names) : gmap term _)) ==∗
+  ∃ names' : gmap term gname,
+  ⌜dom names' = dom names ∪ T⌝ ∗
+  own term_meta_name (● ((to_agree <$> names') : gmap term _)) ∗
+  [∗ set] t ∈ T, term_token t ⊤) as names_alloc.
+{ induction T as [|t T fresh IH] using set_ind_L.
+  - iIntros "%names _ own !>". iExists names.
+    by rewrite right_id_L big_sepS_empty; iFrame.
+  - iIntros "%names %dis own".
+    have t_names : t ∉ dom names by set_solver.
+    have {}dis : dom names ## T by set_solver.
+    iMod gmeta_token_alloc as "(%γ & token)".
+    iMod (own_update with "own") as "[own frag]".
+    { eapply auth_update_alloc.
+      apply (alloc_singleton_local_update _ t (to_agree γ)) => //.
+      by rewrite lookup_fmap (_ : names !! t = None) // -not_elem_of_dom. }
+    rewrite -fmap_insert.
+    have {}dis: dom (<[t := γ]>names) ## T.
+      rewrite dom_insert; set_solver.
+    iMod (IH _ dis with "own") as "(%names' & %dom_names' & own & tokens)".
+    iModIntro. iExists names'. iFrame.
+    rewrite dom_names' dom_insert_L. iSplit; first by iPureIntro; set_solver.
+    rewrite big_sepS_union; last by set_solver.
+    iFrame. rewrite big_sepS_singleton.
+    rewrite term_token_unseal. iExists γ. iFrame. }
+iIntros "PE QE PQ (%names & own & #minted_names)".
+iAssert (⌜dom names ## T⌝)%I as "%dis".
+{ rewrite elem_of_disjoint. iIntros "%t %t_names %t_T".
+  rewrite big_sepS_delete //. iDestruct "minted_names" as "[minted_t _]".
+  iDestruct "PQ" as "[P _]".
+  iApply ("PE" with "[//] P minted_t"). }
+iMod (names_alloc _ dis with "own") as "(%names' & %dom_names & own & tokens)".
+iDestruct "PQ" as "[_ >Q]".
+iAssert ([∗ set] t ∈ T, minted t)%I as "#minted_T".
+{ rewrite (big_sepS_forall _ T). iIntros "%t %t_T".
+  by iApply ("QE" with "[//] Q"). }
+iModIntro. iFrame. rewrite dom_names big_sepS_union //. by iSplit.
+Qed.
+
+Context `{!HasTermMetaCtx ctx}.
+
+Lemma term_token_alloc (T : gset term) (P Q : iProp) E :
+  ↑nroot.@"cryptis".@"meta" ⊆ E →
+  ctx -∗
+  (∀ t, ⌜t ∈ T⌝ -∗ P -∗ minted t -∗ False) -∗
+  (∀ t, ⌜t ∈ T⌝ -∗ Q -∗ minted t) -∗
+  (P ∧ |={E ∖ ↑nroot.@"cryptis".@"meta"}=> Q) ={E}=∗
+  Q ∗ [∗ set] t ∈ T, term_token t ⊤.
+Proof.
+iIntros "%sub ctx H1 H2 H3".
+iPoseProof (has_term_meta_ctx with "ctx") as "{ctx} #ctx".
+iInv "ctx" as ">inv" => //.
+iMod (term_token_alloc_aux with "H1 H2 H3 inv") as "(inv & post & token)".
+iModIntro. by iFrame.
+Qed.
+
+End TermMeta.
+
+Arguments term_token {Σ _} t E.
+Arguments term_meta {Σ _ L _ _} t N x.
+Arguments term_meta_set {Σ _ _ _ _} N x E t.
+Arguments term_token_difference {Σ _} t E1 E2.
+Arguments term_name {Σ _} t γ.
+Arguments term_own {Σ _ A _} t N x.
+Arguments term_own_alloc {Σ _ A _ t} N {_} a.
+Arguments term_own_update {Σ _ A _ t N a} a'.
